defined custom induction principle

Subsumption-STLC.v
@@ -2,6 +2,8 @@
 
 Require Import String.
 Require Import Coq.Strings.String.
+Require Import Coq.Lists.List.
+Import ListNotations.
 Require Coq.MSets.MSetWeakList.
 Module WS := Coq.MSets.MSetWeakList.
 Require Coq.MSets.MSetFacts.
@@ -12,9 +14,52 @@ Require Import Coq.Logic.FunctionalExtensionality.
     
 Definition id := string.
 
+Definition field (t : Type) : Type := id * t.
+
+Definition fields (t : Type) : Type := list (field t).
+
+Definition predf {U : Type} (P : U -> Prop) : field U -> Prop := fun f => P (snd f).
+
+Definition predfs {U : Type} (P : U -> Prop) (fs : fields U) : Prop := Forall (predf P) fs.
+
 Inductive type : Type :=
     | TTop
     | TFun (t t' : type)
-    | TRecord (fields : list (id * type)).
+    | TRec (fs : fields type).
 
-(* Need to define induction principle...yikes... *)
+(* automatically generated induction principle is weak *)
+Check type_ind.
+Compute type_ind.
+Compute type_rect.
+
+(* custom induction principle for Type type *)
+Section TypeInduction.
+    
+    Variable P : type -> Prop.
+
+    Hypothesis HTop : P TTop.
+
+    Hypothesis HFun : forall (t t' : type),
+        P t -> P t' -> P (TFun t t').
+
+    Hypothesis HRec : forall (fs : fields type),
+        predfs P fs -> P (TRec fs).
+
+    Fixpoint IHType (t : type) : P t.
+    Proof.
+        destruct t.
+        - assumption.
+        - apply HFun; apply IHType.
+        - apply HRec. induction fs; constructor.
+            + apply IHType.
+            + assumption.
+    Qed.
+End TypeInduction.
+
+Lemma test_type_ind : forall (t : type), t = t.
+Proof.
+    induction t using IHType.
+    - reflexivity.
+    - constructor.
+    - constructor. (* has correct induction hypothesis! *)
+Qed.
